Massive code cleanup (still more to come)
- Removed old Prover and EProver interfaces
- Ported AssumptionProver and DefaultProver
- Removing old Subst interface
- Removing old implementations of SubstI
- Lemmas inside ExprProp.

theories/ExprProp.v
@@ -1,4 +1,9 @@
 Require Import Coq.Lists.List.
+Require Import ExtLib.Structures.Traversable.
+Require Import ExtLib.Data.List.
+Require Import ExtLib.Data.HList.
+Require Import ExtLib.Data.Eq.
+Require Import ExtLib.Tactics.
 Require Import MirrorCore.TypesI.
 Require Import MirrorCore.ExprI.
 
@@ -7,25 +12,168 @@ Set Strict Implicit.
 
 Section semantic.
   Variable typ : Type.
-  Context {RType_typ : RType typ}.
-  Variable TI_prop : Typ0 _ Prop.
   Variable expr : Type.
+  Context {RType_typ : RType typ}.
   Context {Expr_expr : Expr _ expr}.
+  Context {Typ0_Prop : Typ0 _ Prop}.
 
-  Let tvProp := @typ0 _ _ _ TI_prop.
+  Context {ExprOk_expr : ExprOk _}.
+
+  Let tvProp := @typ0 _ _ _ Typ0_Prop.
 
   Definition Provable_val (val : typD nil tvProp) : Prop :=
     match typ0_cast nil in _ = t return t with
       | eq_refl => val
     end.
 
-  Definition Provable uvars vars (e : expr) : Prop :=
-    match exprD uvars vars e tvProp with
-      | None => False
-      | Some p => Provable_val p
+  Definition Provable tus tvs (e : expr) : ResType tus tvs Prop :=
+    match exprD' tus tvs e tvProp with
+      | None => None
+      | Some p => Some (match typ0_cast nil in _ = t
+                              return HList.hlist _ tus -> HList.hlist _ tvs -> t
+                        with
+                          | eq_refl => p
+                        end)
     end.
 
-  Definition AllProvable uvars vars (es : list expr) :=
-    Forall (Provable uvars vars) es.
+  Theorem Provable_weaken
+  : forall tus tus' tvs tvs' e eD,
+      Provable tus tvs e = Some eD ->
+      exists eD',
+        Provable (tus ++ tus') (tvs ++ tvs') e = Some eD' /\
+        forall us us' vs vs',
+          eD us vs <-> eD' (hlist_app us us') (hlist_app vs vs').
+  Proof.
+    unfold Provable.
+    intros; forward; inv_all; subst.
+    eapply exprD'_weaken with (tus' := tus') (tvs' := tvs') in H; eauto.
+    forward_reason.
+    rewrite H. eexists; split; eauto.
+    intros.
+    repeat first [ rewrite eq_Const_eq | rewrite eq_Arr_eq ].
+    rewrite <- H0. reflexivity.
+  Qed.
+
+  Definition AllProvable tus tvs (es : list expr) : ResType tus tvs Prop :=
+    match mapT (T:=list) (F:=option) (Provable tus tvs) es with
+      | None => None
+      | Some Ps => Some (fun us vs => Forall (fun x => x us vs) Ps)
+    end.
+
+  Theorem AllProvable_nil
+  : forall tus tvs, exists eD,
+      AllProvable tus tvs nil = Some eD /\
+      forall us vs, eD us vs.
+  Proof.
+    compute. intros. eexists; split; auto.
+    constructor.
+  Qed.
+
+  Theorem AllProvable_nil_Some
+  : forall tus tvs eD,
+      AllProvable tus tvs nil = Some eD ->
+      forall us vs, eD us vs.
+  Proof.
+    compute. intros; inv_all; subst. constructor.
+  Qed.
+
+  Theorem AllProvable_cons
+  : forall tus tvs p ps PD,
+      AllProvable tus tvs (p :: ps) = Some PD ->
+      exists pD psD,
+        Provable tus tvs p = Some pD /\
+        AllProvable tus tvs ps = Some psD /\
+        forall us vs,
+          PD us vs <-> (pD us vs /\ psD us vs).
+  Proof.
+    unfold AllProvable.
+    simpl. intros.
+    forward. inv_all; subst.
+    do 2 eexists; split; eauto.
+    split; eauto.
+    simpl. intros.
+    split.
+    { inversion 1; subst; auto. }
+    { constructor; intuition. }
+  Qed.
+
+  Theorem AllProvable_cons'
+  : forall tus tvs p ps pD psD,
+      Provable tus tvs p = Some pD ->
+      AllProvable tus tvs ps = Some psD ->
+      exists PD,
+        AllProvable tus tvs (p :: ps) = Some PD /\
+        forall us vs,
+          PD us vs <-> (pD us vs /\ psD us vs).
+  Proof.
+    unfold AllProvable.
+    simpl. intros.
+    forward. eexists; split; eauto.
+    simpl; intros.
+    inv_all; subst.
+    split.
+    { inversion 1; subst; intuition. }
+    { destruct 1; constructor; auto. }
+  Qed.
+
+  Theorem AllProvable_weaken
+  : forall tus tus' tvs tvs' ps psD,
+      AllProvable tus tvs ps = Some psD ->
+      exists psD',
+        AllProvable (tus ++ tus') (tvs ++ tvs') ps = Some psD' /\
+        forall us us' vs vs',
+          psD us vs <-> psD' (HList.hlist_app us us') (HList.hlist_app vs vs').
+  Proof.
+    induction ps; intros.
+    { eexists; split; [ reflexivity | ].
+      split; intros.
+      { constructor. }
+      { eapply AllProvable_nil_Some in H; eassumption. } }
+    { eapply AllProvable_cons in H.
+      forward_reason.
+      eapply Provable_weaken with (tus' := tus') (tvs' := tvs') in H.
+      eapply IHps in H0.
+      forward_reason.
+      eapply AllProvable_cons' in H0; eauto.
+      forward_reason.
+      eexists; split; eauto.
+      intros.
+      rewrite H1; clear H1.
+      rewrite H3; clear H3.
+      rewrite H2; clear H2.
+      rewrite H4; clear H4. reflexivity. }
+  Qed.
+
+  Theorem AllProvable_app
+  : forall tus tvs p ps pD psD,
+      AllProvable tus tvs p = Some pD ->
+      AllProvable tus tvs ps = Some psD ->
+      exists PD,
+        AllProvable tus tvs (p ++ ps) = Some PD /\
+        forall us vs,
+          PD us vs <-> (pD us vs /\ psD us vs).
+  Proof.
+    intros tus tvs p ps pD psD H H'.
+    generalize dependent pD.
+    induction p.
+    { intros.
+      simpl. eexists; split; eauto.
+      intuition. eapply AllProvable_nil_Some in H; eauto. }
+    { intros.
+      eapply AllProvable_cons in H.
+      forward_reason.
+      eapply IHp in H0.
+      forward_reason.
+      simpl.
+      eapply AllProvable_cons' in H0; eauto.
+      forward_reason.
+      eexists; split; eauto.
+      intros.
+      rewrite H3; rewrite H2; rewrite H1.
+      intuition. }
+  Qed.
 
 End semantic.
+
+Arguments Provable {typ expr RType Expr Typ0} tus tvs e : rename.
+Arguments AllProvable {typ expr RType Expr Typ0} tus tvs es : rename.
