theories/EProver2.v
@@ -1,10 +1,11 @@
-Require Import ExtLib.Structures.Traversable.
 Require Import ExtLib.Data.List.
 Require Import ExtLib.Tactics.
 Require Import MirrorCore.TypesI.
 Require Import MirrorCore.ExprI.
 Require Import MirrorCore.EnvI.
 Require Import MirrorCore.SubstI3.
+Require Import MirrorCore.ExprProp.
+Require Import MirrorCore.Prover2.
 
 Set Implicit Arguments.
 Set Strict Implicit.
@@ -14,17 +15,10 @@ Set Strict Implicit.
  **)
 Section proverI.
   Context {typ : Type}.
-  Context {RType_typ : RType typ}.
   Variable expr : Type.
+  Context {RType_typ : RType typ}.
   Context {Expr_expr : Expr _ expr}.
-  Context {ty : typ}.
-  Variable Provable' : typD nil ty -> Prop.
-
-  Let Provable us vs e :=
-    match exprD us vs e ty with
-      | None => False
-      | Some p => Provable' p
-    end.
+  Context {Typ0_Prop : Typ0 _ Prop}.
 
   Record EProver : Type :=
   { Facts : Type
@@ -47,7 +41,7 @@ Section proverI.
       (forall sumD subD goalD,
          Valid tus tvs sum = Some sumD ->
          substD tus tvs sub = Some subD ->
-         exprD' tus tvs goal ty = Some goalD ->
+         Provable tus tvs goal = Some goalD ->
          exists subD',
            substD tus tvs sub' = Some subD' /\
            forall (us : HList.hlist (typD nil) tus)
@@ -55,44 +49,35 @@ Section proverI.
              sumD us vs ->
              subD' us vs ->
              subD us vs /\
-             Provable' (goalD us vs)).
+             goalD us vs).
 
   Record EProverOk (P : EProver) : Type :=
   { factsD : forall tus tvs : tenv typ, Facts P -> ResType tus tvs Prop
-  ; factsD_weakenU
+  ; factsD_weaken
     : forall tus tvs f sumD,
         factsD tus tvs f = Some sumD ->
-        forall tus',
+        forall tus' tvs',
         exists sumD',
-             factsD (tus ++ tus') tvs f = Some sumD'
-          /\ forall us vs us',
+             factsD (tus ++ tus') (tvs ++ tvs') f = Some sumD'
+          /\ forall us vs us' vs',
                sumD us vs <->
-               sumD' (HList.hlist_app us us') vs
-  ; factsD_weakenV
-    : forall tus tvs f sumD,
-        factsD tus tvs f = Some sumD ->
-        forall tvs',
-        exists sumD',
-             factsD tus (tvs ++ tvs') f = Some sumD'
-          /\ forall us vs vs',
-               sumD us vs <->
-               sumD' us (HList.hlist_app vs vs')
+               sumD' (HList.hlist_app us us') (HList.hlist_app vs vs')
   ; Summarize_sound
     : forall tus tvs hyps premD,
-        mapT (T := list) (F := option) (fun e => exprD' tus tvs e ty) hyps = Some premD ->
+        AllProvable tus tvs hyps = Some premD ->
         exists sumD,
           factsD tus tvs (Summarize P tus tvs hyps) = Some sumD /\
           forall us vs,
-            Forall (fun x => Provable' (x us vs)) premD ->
+            premD us vs ->
             sumD us vs
   ; Learn_sound
     : forall tus tvs hyps premD sum sumD,
         factsD tus tvs sum = Some sumD ->
-        mapT (T := list) (F := option) (fun e => exprD' tus tvs e ty) hyps = Some premD ->
+        AllProvable tus tvs hyps = Some premD ->
         exists sumD',
           factsD tus tvs (Learn P sum tus tvs hyps) = Some sumD' /\
           forall us vs,
-            Forall (fun x => Provable' (x us vs)) premD ->
+            premD us vs ->
             sumD us vs ->
             sumD' us vs
   ; Prove_sound
@@ -100,34 +85,6 @@ Section proverI.
              (Sok : SubstOk _ _),
         EProveOk Sok factsD (@Prove P subst Ssubst)
   }.
-
-(*
-  Theorem Prove_concl P (Pok : EProverOk P)
-  : forall subst (Ssubst : Subst subst expr)
-           (Sok : SubstOk _ _)
-           (vars uvars : env typD)
-           (sum : Facts P),
-      forall (goal : expr) (sub sub' : subst),
-        Prove P sum (typeof_env uvars) (typeof_env vars) sub goal = Some sub' ->
-        WellFormed_subst sub ->
-        WellFormed_subst sub' /\
-        (Valid Pok uvars vars sum ->
-         WellTyped_subst (typeof_env uvars) (typeof_env vars) sub ->
-         WellTyped_subst (typeof_env uvars) (typeof_env vars) sub' /\
-         (substD uvars vars sub' ->
-          forall val,
-            exprD uvars vars goal ty = Some val ->
-            Provable' val /\ substD uvars vars sub)).
-  Proof.
-    intros.
-    destruct (@Pok.(Prove_correct) Sok uvars vars sum goal sub H H0).
-    split; auto.
-    intros. forward_reason. 
-    split; auto.
-    intros. forward_reason.
-    rewrite H7 in *. assumption.
-  Qed.
-*)
 
   (** Composite Prover **)
   Section composite.
@@ -151,8 +108,6 @@ Section proverI.
     Variable pl_correct : EProverOk pl.
     Variable pr_correct : EProverOk pr.
 
-    Opaque mapT.
-
     Theorem composite_ProverT_correct : EProverOk composite_EProver.
     Proof.
       refine (
@@ -166,17 +121,11 @@ Section proverI.
              end
          |}).
       { intros. forward. inv_all; subst.
-        eapply factsD_weakenU with (tus' := tus') in H0.
-        eapply factsD_weakenU with (tus' := tus') in H1.
+        eapply factsD_weaken with (tus' := tus') (tvs' := tvs') in H0.
+        eapply factsD_weaken with (tus' := tus') (tvs' := tvs') in H1.
         forward_reason. Cases.rewrite_all_goal.
         eexists; split; eauto. intros. simpl.
         rewrite <- H2. rewrite H1. reflexivity. }
-      { intros. forward. inv_all; subst.
-        eapply factsD_weakenV with (tvs' := tvs') in H0.
-        eapply factsD_weakenV with (tvs' := tvs') in H1.
-        forward_reason. Cases.rewrite_all_goal.
-        eexists; split; eauto. intros. simpl.
-        rewrite <- H2. rewrite <- H1. reflexivity. }
       { simpl; intros.
         specialize (@Summarize_sound _ pl_correct _ _ _ _ H).
         specialize (@Summarize_sound _ pr_correct _ _ _ _ H).
@@ -215,31 +164,30 @@ Section proverI.
 
   (** From non-EProvers **)
   Section non_eprover.
-    Require Import MirrorCore.Prover2.
     Variables p : @Prover typ expr.
 
     Definition from_Prover : EProver :=
       @Build_EProver
-        p.(Facts)
-        p.(Summarize)
-        p.(Learn)
+        p.(Prover2.Facts)
+        p.(Prover2.Summarize)
+        p.(Prover2.Learn)
         (fun subst Subst facts uenv venv s goal =>
-           if p.(Prove) facts uenv venv goal then Some s else None).
+           if p.(Prover2.Prove) facts uenv venv goal then Some s else None).
 
-    Variable p_correct : ProverOk Provable' p.
+    Variable p_correct : ProverOk p.
 
     Theorem from_ProverT_correct : EProverOk from_Prover.
     Proof.
       refine (
           @Build_EProverOk from_Prover
-                                  p_correct.(factsD) _ _ _ _ _);
+                                  p_correct.(Prover2.factsD) _ _ _ _);
       try solve [ destruct p_correct; simpl; intuition eauto ].
       unfold EProveOk, ProveOk in *.
       intros. simpl in H0.
       simpl in H. forward. inv_all; subst.
       split; auto. intros.
       eexists; split; eauto. intros. split; auto.
-      eapply Prove_sound in H; eauto.
+      eapply Prover2.Prove_sound in H; eauto.
       eapply H; eauto.
     Qed.
   End non_eprover.
