theories/SubstI3.v
@@ -2,11 +2,8 @@ Require Import Coq.Lists.List.
 Require Import ExtLib.Core.RelDec.
 Require Import ExtLib.Structures.Traversable.
 Require Import ExtLib.Data.List.
-Require Import ExtLib.Data.Pair.
-Require Import ExtLib.Data.Nat.
 Require Import ExtLib.Data.HList.
 Require Import ExtLib.Data.Eq.
-Require Import ExtLib.Data.ListNth.
 Require Import ExtLib.Tactics.
 Require Import MirrorCore.TypesI.
 Require Import MirrorCore.ExprI.
